src/SingleValueSim.v
@@ -1,0 +1,155 @@
+Require Import Bool List String Peano_dec.
+Require Import Permutation.
+Require Import Common FMap Syntax Semantics.
+Require Import StepDet StepSeq Predicate Simulation.
+
+Require Import SingleValue.
+
+Set Implicit Arguments.
+
+Open Scope list.
+Open Scope fmap.
+
+Section Sim.
+  Variables extIdx1 extIdx2: nat.
+  Hypotheses (Hiext1: isExternal (impl0 extIdx1 extIdx2) extIdx1 = true)
+             (Hiext2: isExternal (impl0 extIdx1 extIdx2) extIdx2 = true)
+             (Hsext1: isExternal (spec extIdx1 extIdx2) extIdx1 = true)
+             (Hsext2: isExternal (spec extIdx1 extIdx2) extIdx2 = true).
+
+  Local Notation impl0 := (impl0 extIdx1 extIdx2).
+  Local Notation spec := (spec extIdx1 extIdx2).
+
+  Definition svmImplChild1Inv: list (OState -> Prop) :=
+    (fun iost1 => (ost_st iost1)@[statusIdx] = Some (VNat stI))
+      :: (fun iost1 => (ost_st iost1)@[statusIdx] = Some (VNat stS)) 
+      :: (fun iost1 => (ost_st iost1)@[statusIdx] = Some (VNat stM))
+      :: nil.
+
+  Definition svmImplChild2Inv: list (OState -> Prop) :=
+    (fun iost1 => (ost_st iost1)@[statusIdx] = Some (VNat stI))
+      :: (fun iost1 => (ost_st iost1)@[statusIdx] = Some (VNat stS)) 
+      :: (fun iost1 => (ost_st iost1)@[statusIdx] = Some (VNat stM))
+      :: nil.
+
+  Definition svmImplInv: list (ObjectStates -> Prop) :=
+    (fun ioss =>
+       exists iost1 iost2,
+         ioss@[child1Idx] = Some iost1 /\
+         (ost_st iost1)@[statusIdx] = Some (VNat stS) /\
+         ioss@[child2Idx] = Some iost2 /\
+         (ost_st iost2)@[statusIdx] = Some (VNat stS))
+      :: (fun ioss =>
+            exists iost1 iost2,
+              ioss@[child1Idx] = Some iost1 /\
+              (ost_st iost1)@[statusIdx] = Some (VNat stM) /\
+              ioss@[child2Idx] = Some iost2 /\
+              (ost_st iost2)@[statusIdx] = Some (VNat stI))
+      :: (fun ioss =>
+            exists iost1 iost2,
+              ioss@[child1Idx] = Some iost1 /\
+              (ost_st iost1)@[statusIdx] = Some (VNat stI) /\
+              ioss@[child2Idx] = Some iost2 /\
+              (ost_st iost2)@[statusIdx] = Some (VNat stM))
+      :: nil.
+
+  Definition svmR: list (ObjectStates -> ObjectStates -> Prop) :=
+    (fun ioss soss =>
+       exists iost1 iost2 sost v,
+         ioss@[child1Idx] = Some iost1 /\
+         (ost_st iost1)@[statusIdx] = Some (VNat stS) /\
+         (ost_st iost1)@[valueIdx] = Some v /\
+         ioss@[child2Idx] = Some iost2 /\
+         (ost_st iost2)@[statusIdx] = Some (VNat stS) /\
+         (ost_st iost2)@[valueIdx] = Some v /\
+         soss@[specIdx] = Some sost /\
+         (ost_st sost)@[valueIdx] = Some v)
+      :: (fun ioss soss =>
+            exists iost1 iost2 sost v,
+              ioss@[child1Idx] = Some iost1 /\
+              (ost_st iost1)@[statusIdx] = Some (VNat stM) /\
+              (ost_st iost1)@[valueIdx] = Some v /\
+              ioss@[child2Idx] = Some iost2 /\
+              (ost_st iost2)@[statusIdx] = Some (VNat stI) /\
+              soss@[specIdx] = Some sost /\
+              (ost_st sost)@[valueIdx] = Some v)
+      :: (fun ioss soss =>
+            exists iost1 iost2 sost v,
+              ioss@[child1Idx] = Some iost1 /\
+              (ost_st iost1)@[statusIdx] = Some (VNat stI) /\
+              ioss@[child2Idx] = Some iost2 /\
+              (ost_st iost2)@[statusIdx] = Some (VNat stM) /\
+              (ost_st iost2)@[valueIdx] = Some v /\
+              soss@[specIdx] = Some sost /\
+              (ost_st sost)@[valueIdx] = Some v)
+      :: nil.
+
+  Inductive SvmR: ObjectStates -> ObjectStates -> Prop :=
+  | SvmSS: forall ioss soss iost1 iost2 sost v,
+      ioss@[child1Idx] = Some iost1 ->
+      (ost_st iost1)@[statusIdx] = Some (VNat stS) ->
+      (ost_st iost1)@[valueIdx] = Some v ->
+      ioss@[child2Idx] = Some iost2 ->
+      (ost_st iost2)@[statusIdx] = Some (VNat stS) ->
+      (ost_st iost2)@[valueIdx] = Some v ->
+      soss@[specIdx] = Some sost ->
+      (ost_st sost)@[valueIdx] = Some v ->
+      SvmR ioss soss
+  | SvmIM1: forall ioss soss iost1 iost2 sost v,
+      ioss@[child1Idx] = Some iost1 ->
+      (ost_st iost1)@[statusIdx] = Some (VNat stM) ->
+      (ost_st iost1)@[valueIdx] = Some v ->
+      ioss@[child2Idx] = Some iost2 ->
+      (ost_st iost2)@[statusIdx] = Some (VNat stI) ->
+      soss@[specIdx] = Some sost ->
+      (ost_st sost)@[valueIdx] = Some v ->
+      SvmR ioss soss
+  | SvmIM2: forall ioss soss iost1 iost2 sost v,
+      ioss@[child1Idx] = Some iost1 ->
+      (ost_st iost1)@[statusIdx] = Some (VNat stI) ->
+      ioss@[child2Idx] = Some iost2 ->
+      (ost_st iost2)@[statusIdx] = Some (VNat stM) ->
+      (ost_st iost2)@[valueIdx] = Some v ->
+      soss@[specIdx] = Some sost ->
+      (ost_st sost)@[valueIdx] = Some v ->
+      SvmR ioss soss.
+
+  Lemma svmR_svmR:
+    forall ioss soss,
+      SvmR ioss soss ->
+      exists n, nth n svmR (fun _ _ => False) ioss soss.
+  Proof.
+    intros; inv H.
+    - exists 0; cbn.
+      repeat eexists; eauto.
+    - exists 1; cbn.
+      repeat eexists; eauto.
+    - exists 2; cbn.
+      repeat eexists; eauto.
+  Qed.      
+
+  Definition SvmSim (ist sst: TState) := SvmR (tst_oss ist) (tst_oss sst).
+
+  Definition svmIdxF (idx: IdxT): IdxT :=
+    if idx ?<n (indicesOf impl0) then specIdx else idx.
+
+  Definition svmMsgIdF (imid: MsgId): MsgId :=
+    {| mid_type := mid_type imid;
+       mid_from := svmIdxF (mid_from imid);
+       mid_to := svmIdxF (mid_to imid);
+       mid_chn := mid_to imid |}.
+
+  Definition svmMsgF (imsg: Msg): Msg :=
+    {| msg_id := svmMsgIdF (msg_id imsg);
+       msg_value := msg_value imsg |}.
+
+  Definition svmMsgsF (imsgs: list Msg): list Msg :=
+    map svmMsgF imsgs.
+
+  Definition svmP (l: Label) :=
+    match l with
+    | Lbl min mouts => Lbl min (svmMsgsF mouts)
+    end.
+  
+End Sim.
+
