src/SingleValueSyn.v
@@ -1,0 +1,183 @@
+Require Import Bool List String Peano_dec.
+Require Import Permutation.
+Require Import Common FMap Syntax Semantics.
+Require Import StepDet StepSeq Serial Predicate Synthesis.
+
+Require Import SingleValue SingleValueSim.
+
+Set Implicit Arguments.
+
+Open Scope list.
+Open Scope fmap.
+
+Section Impl.
+  Variables extIdx1 extIdx2: nat.
+  Hypotheses (Hiext1: isExternal (impl0 extIdx1 extIdx2) extIdx1 = true)
+             (Hiext2: isExternal (impl0 extIdx1 extIdx2) extIdx2 = true)
+             (Hsext1: isExternal (spec extIdx1 extIdx2) extIdx1 = true)
+             (Hsext2: isExternal (spec extIdx1 extIdx2) extIdx2 = true).
+
+  Local Definition spec := spec extIdx1 extIdx2.
+  Local Definition specObj := specObj extIdx1 extIdx2.
+  Local Definition impl0 := impl0 extIdx1 extIdx2.
+  Local Definition svmP := svmP extIdx1 extIdx2.
+
+  (** First, prove that the initial system is provided properly. *)
+  Theorem impl0_ok: SynthOk spec SvmSim svmP impl0.
+  Proof.
+    repeat split.
+    - admit.
+    - repeat econstructor.
+    - admit.
+  Admitted.
+  
+  Section SynStep.
+
+    Local Definition targetObjIdx := child1Idx.
+    Local Definition targetTrsIdx := 0.
+
+    Ltac get_target_trs impl oidx tidx :=
+      let oobj := (eval cbn in (nth_error (sys_objs impl) oidx)) in
+      match oobj with
+      | Some ?obj =>
+        let otrs := (eval cbn in (nth_error (obj_trs obj) tidx)) in
+        match otrs with
+        | Some ?trs => exact trs
+        end
+      end.
+
+    Ltac cbner t := let ct := (eval cbn in t) in exact ct.
+
+    Ltac get_precond trs :=
+      cbner (pmsg_precond trs).
+    
+    Local Definition targetTrs: PMsg :=
+      ltac:(get_target_trs impl0 targetObjIdx targetTrsIdx).
+
+    Local Definition targetMid: MsgId := pmsg_mid targetTrs.
+    Local Definition targetSpecMid := svmMsgIdF extIdx1 extIdx2 targetMid.
+    Local Definition targetPrec: PreCond := ltac:(get_precond targetTrs).
+
+    Ltac mv_rewriter :=
+      repeat
+        match goal with
+        | [H: Some _ = M.find _ _ |- _] => apply eq_sym in H
+        | [H: None = M.find _ _ |- _] => apply eq_sym in H
+        | [H1: M.find ?m ?k1 = Some _, H2: M.find ?m ?k2 = Some _ |- _] =>
+          rewrite H1 in H2; inv H2
+        | [H1: M.find ?m ?k1 = Some _, H2: M.find ?m ?k2 = None |- _] =>
+          rewrite H1 in H2; discriminate
+        end.
+
+    (* If it succeeds, then provably [inv1] and [inv2] are not compatible 
+     * for all state.
+     * If it fails, then there's no information.
+     *)
+    Ltac inv_not_compatible inv1 inv2 :=
+      let Hnc := fresh "Hnc" in
+      assert (forall st, inv1 st -> inv2 st -> False)
+        as Hnc by (cbn; intros; dest; intuition mv_rewriter);
+      clear Hnc.
+
+    Ltac find_new_prec cprec invs :=
+      match invs with
+      | nil => fail
+      | ?inv :: ?invs' =>
+        tryif (inv_not_compatible cprec inv)
+        then (exact inv)
+        else find_new_prec cprec invs'
+      end.
+
+    Local Definition newPrec: PreCond :=
+      ltac:(let tgt := (eval hnf in targetPrec) in
+            let invs := (eval hnf in svmImplChild1Inv) in
+            find_new_prec tgt invs).
+
+    Ltac find_state_sim oidx oinv sims :=
+      match sims with
+      | nil => fail
+      | ?sim :: ?sims' =>
+        tryif (inv_not_compatible oinv
+                                  (fun iost => exists ist sst,
+                                       ist@[oidx] = Some iost /\ sim ist sst))
+        then find_state_sim oidx oinv sims'
+        else exact sim
+      end.
+
+    Local Definition newStateInv: ObjectStates -> ObjectStates -> Prop :=
+      ltac:(let tgt := (eval hnf in newPrec) in
+            let sims := (eval hnf in svmR) in
+            find_state_sim child1Idx tgt sims).
+
+    Local Definition targetStateInv: ObjectStates -> ObjectStates -> Prop :=
+      ltac:(let tgt := (eval hnf in targetPrec) in
+            let sims := (eval hnf in svmR) in
+            find_state_sim child1Idx tgt sims).
+
+    Local Definition diffs: list VDiff.
+    Proof.
+      pose newStateInv as pre; hnf in pre.
+      pose targetStateInv as post; hnf in post.
+
+    Abort.
+    
+    
+    (* Ltac no_vloc_st oss oidx kidx := *)
+    (*   lazymatch goal with *)
+    (*   | [vloc := (oss, VFromState oidx kidx, _) |- _] => fail *)
+    (*   | _ => idtac *)
+    (*   end. *)
+
+    (* (* NOTE: there's only one [VFromMsg] information per a transaction. *) *)
+    (* Ltac no_vloc_msg := *)
+    (*   lazymatch goal with *)
+    (*   | [vloc := (VFromMsg, _) |- _] => fail *)
+    (*   | _ => idtac *)
+    (*   end. *)
+
+    (* Ltac collect_vloc := *)
+    (*   repeat *)
+    (*     match goal with *)
+    (*     | [H1: M.find ?oidx ?oss = Some ?ost, H2: M.find ?kidx (ost_st ?ost) = Some ?v |- _] => *)
+    (*       no_vloc_st oss oidx kidx; *)
+    (*       let vloc := fresh "vloc" in *)
+    (*       set (oss, VFromState oidx kidx, v) as vloc *)
+    (*     | [H: pmsg_postcond _ _ ?v _ |- _] => *)
+    (*       no_vloc_msg; *)
+    (*       let vloc := fresh "vloc" in *)
+    (*       set (VFromMsg, v) as vloc *)
+    (*     end. *)
+
+    (* Ltac simpl_postcond := *)
+    (*   repeat *)
+    (*     match goal with *)
+    (*     | [H: pmsg_postcond _ _ _ _ |- _] => simpl in H; mv_rewriter *)
+    (*     end. *)
+
+    (* Ltac no_diff sdf := *)
+    (*   lazymatch goal with *)
+    (*   | [df := sdf |- _] => fail *)
+    (*   | _ => idtac *)
+    (*   end. *)
+
+    (* Ltac collect_diff oss1 oss2 := *)
+    (*   repeat *)
+    (*     match goal with *)
+    (*     | [vloc := (oss2, ?wh, ?v) |- _] => *)
+    (*       is_pure_const v; *)
+    (*       no_diff (ConstDiff wh v); *)
+    (*       let df := fresh "df" in *)
+    (*       pose (ConstDiff wh v) as df *)
+    (*     | [vloc1 := (oss1, ?wh1, ?v), vloc2 := (oss2, ?wh2, ?v) |- _] => *)
+    (*       not_pure_const v; *)
+    (*       first [is_equal wh1 wh2 | *)
+    (*              no_diff (VMoved wh1 wh2); *)
+    (*              let df := fresh "df" in *)
+    (*              pose (VMoved wh1 wh2) as df] *)
+    (*     end. *)
+
+    
+  End SynStep.
+
+End Impl.
+
